\documentclass{article}
\usepackage[utf8]{inputenc}
\usepackage{amsmath,amssymb}
\usepackage{enumitem}
\usepackage{graphicx,tikz}
\usepackage{geometry}

\geometry{margin=1in}
\pagestyle{empty}
\setlength{\parindent}{0pt}

\newcommand{\code}[1]{{\fontfamily{pcr}\selectfont #1}}
\newcommand{\abs}[1]{\left|#1\right|}
\newcommand{\srs}[1]{\{#1\}_1^\infty}
\newcommand{\floor}[1]{\left\lfloor#1\right\rfloor}
\newcommand{\ceil}[1]{\left\lceil#1\right\rceil}

\newcommand{\env}[2]{\begin{#1}#2\end{#1}}
\newcommand{\spl}[1]{\begin{split}#1\end{split}}
\newcommand{\mat}[1]{\begin{bmatrix}#1\end{bmatrix}}

\newcommand{\zee}{\mathbb{Z}}
\newcommand{\Q}{\mathbb{Q}}
\newcommand{\arr}{\mathbb{R}}
\newcommand{\C}{\mathbb{C}}
\newcommand{\N}{\mathbb{N}}

\begin{document}

$D = A \cap C$

$A' = A - D$

$C' = C - D$
\[\begin{split}
    (A \oplus_k B) \oplus_k C
    &= ((A' \oplus_k D) \oplus_k B) \oplus_k (D \oplus_k C') \\
    &= (A' \oplus_k (D \oplus_k B)) \oplus_k (D \oplus_k C') \\
    &= ((A' \oplus_k (D \oplus_k B)) \oplus_k D) \oplus_k C' \\
    &= (D \oplus_k (A' \oplus_k (D \oplus_k B))) \oplus_k C' \\
    &= ((D \oplus_k A') \oplus_k (D \oplus_k B)) \oplus_k C' \\
    &= ((A' \oplus_k D) \oplus_k (D \oplus_k B)) \oplus_k C' \\
    &= (A' \oplus_k (D \oplus_k (D \oplus_k B))) \oplus_k C' \\
    &= C' \oplus_k (A' \oplus_k (D \oplus_k (D \oplus_k B))) \\
\end{split}\]

\end{document}
